start proving Derek's contradiction

program_logic/counter_examples.v
@@ -58,3 +58,165 @@ Section savedprop.
     rewrite -uPred.later_intro. apply rvs_false.
   Qed.
 End savedprop.
+
+(** This proves that we need the ▷ when opening invariants. *)
+(** We fork in [uPred M] for any M, but the proof would work in any BI. *)
+Section inv.
+  Context (M : ucmraT).
+  Notation iProp := (uPred M).
+  Notation "¬ P" := (□ (P → False))%I : uPred_scope.
+  Implicit Types P : iProp.
+
+  (** Assumptions *)
+  (* We have view shifts (two classes: empty/full mask) *)
+  Context (pvs0 pvs1 : iProp → iProp).
+
+  Hypothesis pvs0_intro : forall P, P ⊢ pvs0 P.
+
+  Hypothesis pvs0_mono : forall P Q, (P ⊢ Q) → pvs0 P ⊢ pvs0 Q.
+  Hypothesis pvs0_pvs0 : forall P, pvs0 (pvs0 P) ⊢ pvs0 P.
+  Hypothesis pvs0_frame_l : forall P Q, P ★ pvs0 Q ⊢ pvs0 (P ★ Q).
+
+  Hypothesis pvs1_mono : forall P Q, (P ⊢ Q) → pvs1 P ⊢ pvs1 Q.
+  Hypothesis pvs1_pvs1 : forall P, pvs1 (pvs1 P) ⊢ pvs1 P.
+  Hypothesis pvs1_frame_l : forall P Q, P ★ pvs1 Q ⊢ pvs1 (P ★ Q).
+
+  Hypothesis pvs0_pvs1 : forall P, pvs0 P ⊢ pvs1 P.
+
+  (* We have invariants *)
+  Context (name : Type) (inv : name → iProp → iProp).
+  Hypothesis inv_persistent : forall i P, PersistentP (inv i P).
+  Hypothesis inv_alloc_dep :
+    forall (P : name → iProp), (∀ i, P i) ⊢ pvs1 (∃ i, inv i (P i)).
+  Hypothesis inv_open :
+    forall i P Q R, (P ★ Q ⊢ pvs0 (P ★ R)) → (inv i P ★ Q ⊢ pvs1 R).
+
+  (* We have tokens for a little "two-state STS" *)
+  Context (start finished : iProp).
+  Hypothesis start_finish : start ⊢ pvs0 finished.
+  Hypothesis finish_no_start : finished ★ start ⊢ False.
+  Hypothesis finish_persistent : PersistentP finished.
+
+  (** Some general lemmas and proof mode compatibility. *)
+  Lemma inv_open' i P R:
+    inv i P ★ (P -★ pvs0 (P ★ pvs1 R)) ⊢ pvs1 R.
+  Proof.
+    iIntros "(#HiP & HP)". iApply pvs1_pvs1. iApply inv_open; last first.
+    { iSplit; first done. iExact "HP". }
+    iIntros "(HP & HPw)". by iApply "HPw".
+  Qed.
+
+  Lemma pvs1_intro P : P ⊢ pvs1 P.
+  Proof. rewrite -pvs0_pvs1. apply pvs0_intro. Qed.
+
+  Instance pvs0_mono' : Proper ((⊢) ==> (⊢)) pvs0.
+  Proof. intros ?**. by apply pvs0_mono. Qed.
+  Instance pvs0_proper : Proper ((⊣⊢) ==> (⊣⊢)) pvs0.
+  Proof.
+    intros P Q Heq.
+    apply (anti_symm (⊢)); apply pvs0_mono; by rewrite ?Heq -?Heq.
+  Qed.
+  Instance pvs1_mono' : Proper ((⊢) ==> (⊢)) pvs1.
+  Proof. intros ?**. by apply pvs1_mono. Qed.
+  Instance pvs1_proper : Proper ((⊣⊢) ==> (⊣⊢)) pvs1.
+  Proof.
+    intros P Q Heq.
+    apply (anti_symm (⊢)); apply pvs1_mono; by rewrite ?Heq -?Heq.
+  Qed.
+
+  Lemma pvs0_frame_r : forall P Q, (pvs0 P ★ Q) ⊢ pvs0 (P ★ Q).
+  Proof.
+    intros. rewrite comm pvs0_frame_l. apply pvs0_mono. by rewrite comm.
+  Qed.
+  Lemma pvs1_frame_r : forall P Q, (pvs1 P ★ Q) ⊢ pvs1 (P ★ Q).
+  Proof.
+    intros. rewrite comm pvs1_frame_l. apply pvs1_mono. by rewrite comm.
+  Qed.
+
+  Global Instance elim_pvs0_pvs0 P Q :
+    ElimVs (pvs0 P) P (pvs0 Q) (pvs0 Q).
+  Proof.
+    rename Q0 into Q.
+    rewrite /ElimVs. etrans; last eapply pvs0_pvs0.
+    rewrite pvs0_frame_r. apply pvs0_mono. by rewrite uPred.wand_elim_r.
+  Qed.
+
+  Global Instance elim_pvs1_pvs1 P Q :
+    ElimVs (pvs1 P) P (pvs1 Q) (pvs1 Q).
+  Proof.
+    rename Q0 into Q.
+    rewrite /ElimVs. etrans; last eapply pvs1_pvs1.
+    rewrite pvs1_frame_r. apply pvs1_mono. by rewrite uPred.wand_elim_r.
+  Qed.
+
+  Global Instance elim_pvs0_pvs1 P Q :
+    ElimVs (pvs0 P) P (pvs1 Q) (pvs1 Q).
+  Proof.
+    rename Q0 into Q.
+    rewrite /ElimVs. rewrite pvs0_pvs1. apply elim_pvs1_pvs1.
+  Qed.
+
+  (** Now to the actual counterexample. *)
+  Definition saved (i : name) (P : iProp) : iProp :=
+    inv i (start ∨ □P ★ finished).
+
+  Lemma saved_alloc (P : name → iProp) :
+    start ⊢ pvs1 (∃ i, saved i (P i)).
+  Proof.
+    iIntros "HS". iApply inv_alloc_dep. iIntros (?). by iLeft.
+  Qed.
+
+  Lemma saved_agree i P Q :
+    saved i P ★ saved i Q ★ □P ⊢ pvs1 (□Q).
+  Proof.
+    iIntros "(#HsP & #HsQ & #HP)". iApply (inv_open' i). iSplit; first iExact "HsP".
+    iIntros "HiP". iAssert (pvs0 (□P  ★ finished)) with "[HiP]" as "Hf".
+    { iDestruct "HiP" as "[Hs | [_ Hf]]".
+      - iApply pvs0_frame_l. iSplit; first done. by iApply start_finish.
+      - iApply pvs0_intro. iSplit; done. }
+    iVs "Hf" as "[_ #Hf]". iApply pvs0_intro. iSplitL.
+    { iRight. eauto. }
+    iApply (inv_open' i). iSplit; first iExact "HsQ".
+    iIntros "[Hs | [#HQ _]]".
+    { iExFalso. iApply finish_no_start. eauto. }
+    iApply pvs0_intro. iSplitL.
+    { iRight. eauto. }
+    iApply pvs1_intro. done.
+  Qed.
+
+(*
+Now, define:
+
+N(P) :=  box(P ==> False)
+A[i] :=  Exists P. N(P) * i |-> P
+
+Notice that A[i] => box(A[i]).
+
+OK, now we are going to prove that True ==> False.
+
+First we allocate some k s.t. k |-> A[k], which we know we can do
+because of the axiom for |->.
+
+Claim 2: N(A[k]).
+
+Proof:
+- Suppose A[k].  So, box(A[k]).  So, A[k] * A[k].
+- So there is some P s.t. A[k] * N(P) * k |-> P.
+- Since k |-> A(k), by Claim 1 we can view shift to P * N(P).
+- Hence, we can view shift to False.
+QED.
+
+Notice that in Iris proper all we could get on the third line of the
+above proof is later(P) * N(P), which would not be enough to derive
+the claim.
+
+Claim 3: A[k].
+
+Proof:
+- By Claim 2, we have N(A(k)) * k |-> A[k].
+- Thus, picking P := A[k], we have Exists P. N(P) * k |-> P, i.e. we have A[k].
+QED.
+
+Claim 2 and Claim 3 together view shift to False.
+*)
+End inv.
